impredicative_set/ifmt_lifting.v
@@ -217,40 +217,6 @@ by rewrite compA -K_opE.
 Qed.
 End theorem27.
 
-Section proposition_28.
-
-Variables (E : functor) (M : monad) (aop : E.-aoperation M) (t : FMT).
-Hypothesis naturality_k_type : forall (A : UU0) (m : k_type M A),
-  naturality_k_type m.
-
-Lemma proposition_28 :
-  hlifting aop t naturality_k_type = alifting aop (Lift t M).
-Proof.
-rewrite /hlifting /K_op.
-rewrite {1}/alifting.
-rewrite psiK.
-rewrite /alifting.
-apply/nattrans_ext => A.
-rewrite 2!vcompE.
-rewrite functor_app_naturalE.
-rewrite 2!psiE.
-rewrite vcompE.
-transitivity (
-(Hmap t (from naturality_k_type) A \o
-     Join \o monadM_nt (Lift t (K_MonadT M)) (t (K_MonadT M) A)) \o (kappa aop (t (K_MonadT M) A) \o
-    E # Hmap t (monadM_nt (Lift K_MonadT M)) A)
-) => //.
-rewrite -natural.
-transitivity (
-  (Hmap t (from naturality_k_type) A \o Join) \o (monadM_nt (Lift t (K_MonadT M)) (t (K_MonadT M) A) \o
-    (K_MonadT M # Hmap t (monadM_nt (Lift K_MonadT M)) A) \o kappa aop (t M A))
-) => //.
-rewrite -natural.
-rewrite kappaE vcompE phiE.
-Abort.
-
-End proposition_28.
-
 Section example_29_stateT.
 Variables (E : functor) (M : monad) (op : E.-operation M).
 Hypothesis naturality_k_type : forall (A : UU0) (m : k_type M A),
@@ -417,10 +383,122 @@ Qed.
 
 End example_29_outputT.
 
+Section proposition_28_stateFMT.
+
+Variables (E : functor) (M : monad) (aop : E.-aoperation M).
+Hypothesis naturality_k_type : forall (A : UU0) (m : k_type M A),
+  naturality_k_type m.
+
+Lemma proposition_28_stateFMT (S : UU0) (t := stateFMT S) :
+  hlifting aop t naturality_k_type = alifting aop (Lift t M).
+Proof.
+apply nattrans_ext => X.
+rewrite (hlifting_stateT aop naturality_k_type S).
+apply fun_ext => m.
+apply fun_ext => s.
+rewrite /alifting.
+rewrite psiE /= /bindS -liftSE /liftS /=.
+rewrite 2!algebraic.
+congr (aop _ _).
+rewrite -[RHS](compE _ (E # _)).
+rewrite -functor_o.
+rewrite -[RHS](compE _ (E # _)).
+rewrite -functor_o.
+congr ((E # _) m).
+apply fun_ext => x.
+by rewrite /= 2!bindretf.
+Qed.
+
+End proposition_28_stateFMT.
+
+Section example_30.
+Variable Env : UU0.
+Let E := imonad_model.EnvironmentOps.Local.func Env.
+Let M := imonad_model.ModelMonad.Environment.t Env.
+Let local : E.-operation M := imonad_model.EnvironmentOps.local_op Env.
+Hypothesis naturality_k_type : forall (A : UU0) (m : k_type M A),
+  naturality_k_type m.
+
+Section example_30_FMT.
+Variable T : FMT.
+
+Definition localKT (X : UU0) (f : Env -> Env) (t : T (K_MonadT M) X) : T (K_MonadT M) X :=
+  Join (Lift T (K_MonadT M) (T (K_MonadT M) X) (fun Y k => local Y (f, k t))).
+
+Definition localT (X : UU0) (f : Env -> Env) (t : T M X) : T M X :=
+  let t' := Hmap T (monadM_nt (Lift K_MonadT M)) X t in
+  Hmap T (from naturality_k_type) X (localKT f t').
+
+End example_30_FMT.
+
+Section example_30_stateT.
+Variable S : UU0.
+
+Definition local_stateT (X : UU0) (f : Env -> Env) (t : stateFMT S M X) : stateFMT S M X := fun s e => t s (f e).
+
+Let local_stateT' (X : UU0) : (E \O stateFMT S M) X -> (stateFMT S M) X :=
+  uncurry (@local_stateT X).
+
+Lemma local_stateTE (X : UU0) :
+  (hlifting local (stateFMT S) naturality_k_type) X = @local_stateT' X.
+Proof.
+rewrite hlifting_stateT.
+by apply fun_ext => -[].
+Qed.
+End example_30_stateT.
+
+Section example_30_errorT.
+Variable Z : UU0.
+Definition local_errorT (X : UU0) (f : Env -> Env) (t : errorFMT Z M X) : errorFMT Z M X := fun e => t (f e).
+
+Let local_errorT' (X : UU0) : (E \O errorFMT Z M) X -> (errorFMT Z M) X :=
+  uncurry (@local_errorT X).
+
+Lemma local_errorTE (X : UU0) :
+  (hlifting local (errorFMT Z) naturality_k_type) X = @local_errorT' X.
+Proof.
+rewrite hlifting_errorT.
+by apply fun_ext => -[].
+Qed.
+
+End example_30_errorT.
+
+Section example_31_envT.
+Variable Z : UU0.
+Definition local_envT (X : UU0) (f : Env -> Env) (t : envFMT Z M X) : envFMT Z M X := fun e e' => t e (f e').
+
+Let local_envT' (X : UU0) : (E \O envFMT Z M) X -> (envFMT Z M) X :=
+  uncurry (@local_envT X).
+
+Lemma local_envTE (X : UU0) :
+  (hlifting local (envFMT Z) naturality_k_type) X = @local_envT' X.
+Proof.
+rewrite hlifting_envT.
+by apply fun_ext => -[].
+Qed.
+End example_31_envT.
+
+Section example_31_outputT.
+Variable R : UU0.
+Definition local_outputT (X : UU0) (f : Env -> Env) (t : outputFMT R M X) : outputFMT R M X := fun e => t (f e).
+
+Let local_outputT' (X : UU0) : (E \O outputFMT R M) X -> (outputFMT R M) X :=
+  uncurry (@local_outputT X).
+
+Lemma local_outputTE (X : UU0) :
+  (hlifting local (outputFMT R) naturality_k_type) X = @local_outputT' X.
+Proof.
+rewrite hlifting_outputT.
+by apply fun_ext; case.
+Qed.
+End example_31_outputT.
+
+End example_30.
+
 Section example_31. (* error monad with Z = unit *)
 Let E := imonad_model.ExceptOps.Handle.func unit.
 Let M := imonad_model.ModelExcept.t.
-Let handle : E.-operation M:= @imonad_model.ExceptOps.handle_op unit.
+Let handle : E.-operation M := @imonad_model.ExceptOps.handle_op unit.
 Hypothesis naturality_k_type : forall (A : UU0) (m : k_type M A),
   naturality_k_type m.
 
@@ -503,3 +581,61 @@ Qed.
 End example_31_outputT.
 
 End example_31.
+
+Section example_32.
+Variable R : UU0.
+Let E := imonad_model.OutputOps.Flush.func.
+Let M := imonad_model.ModelMonad.Output.t R.
+Let flush : E.-operation M := @imonad_model.OutputOps.flush_op R.
+Hypothesis naturality_k_type : forall (A : UU0) (m : k_type M A),
+  naturality_k_type m.
+
+Section example_32_stateT.
+Variable S : UU0.
+Definition flush_stateT (X : UU0) (t : stateFMT S M X) : stateFMT S M X := fun s => let: (x, _) := t s in (x, [::]).
+
+Lemma flush_stateTE (X : UU0) :
+  (hlifting flush (stateFMT S) naturality_k_type) X = @flush_stateT X.
+Proof. by rewrite hlifting_stateT. Qed.
+End example_32_stateT.
+
+Section example_32_errorT.
+Variable Z : UU0.
+Definition flush_errorT (X : UU0) (t : errorFMT Z M X) (h : Z -> errorFMT Z M X) : errorFMT Z M X :=
+  let: (c, _) := t in (c, [::]).
+
+Let flush_errorT' (X : UU0) : (E \O errorFMT Z M) X -> (errorFMT Z M) X :=
+  fun c => let : (x, _) := c in (x, [::]).
+
+Lemma flush_errorTE (X : UU0) :
+  (hlifting flush (errorFMT Z) naturality_k_type) X = @flush_errorT' X.
+Proof. by rewrite hlifting_errorT. Qed.
+End example_32_errorT.
+
+Section example_32_envT.
+Variable Z : UU0.
+Definition flush_envT (X : UU0) (t : envFMT Z M X) : envFMT Z M X :=
+  fun e => let: (x, _) := t e in (x, [::]).
+
+Lemma flush_envTE (X : UU0) :
+  (hlifting flush (envFMT Z) naturality_k_type) X = @flush_envT X.
+Proof. by rewrite hlifting_envT. Qed.
+End example_32_envT.
+
+Section example_32_outputT.
+Variable Z : UU0.
+Definition flush_outputT (X : UU0) (t : outputFMT R M X) (h : Z -> outputFMT R M X)
+  : outputFMT R M X := let: (p, w) := t in (p, [::]).
+
+Let flush_outputT' (X : UU0) : (E \O outputFMT R M) X -> (outputFMT R M) X :=
+  fun e => let: (pw, w') := e in (pw, [::]).
+
+Lemma flush_outputTE (X : UU0) :
+  (hlifting flush (outputFMT R) naturality_k_type) X = @flush_outputT' X.
+Proof.
+rewrite hlifting_outputT.
+by apply fun_ext; case.
+Qed.
+End example_32_outputT.
+
+End example_32.
